HMAC_spec_parameters.v
@@ -1,0 +1,49 @@
+  (* c is the output size, b is the block size 
+     (larger than the output size),
+     and p is the difference between them *)
+  Variable c p : nat.
+  Definition b := c + p.
+  
+  (* compression function *)
+  Variable h : Bvector c -> Bvector b -> Bvector c.
+
+  (* initialization vector *)
+  Variable iv : Bvector c.
+
+  Variable splitAndPad : Blist -> list (Bvector b).
+  
+  Variable fpad : Bvector c -> Bvector p. 
+  Definition app_fpad (x : Bvector c) : Bvector b :=
+    (Vector.append x (fpad x)).
+
+  Variable opad ipad : Bvector b.
+
+  (* ----- Definitions *)
+
+  (* The iteration of the compression function gives a keyed hash function on lists of words. *)
+  Definition h_star k (m : list (Bvector b)) :=
+    fold_left h m k.
+
+  (* The composition of the keyed hash function with the IV gives a hash function on lists of words. *)
+  Definition hash_words := h_star iv.
+
+  (* ----- Instantiation *)
+
+  Definition c := (SHA256_.DigestLength * 8)%nat.
+  Definition p := (32 * 8)%nat.
+
+  Definition intsToBits (l : list int) : list bool :=
+    bytesToBits (SHA256.intlist_to_Zlist l).
+
+  Definition bitsToInts (l : Blist) : list int :=
+    SHA256.Zlist_to_intlist (bitsToBytes l).
+
+  Definition sha_iv : Blist :=
+    intsToBits SHA256.init_registers.
+
+  Definition sha_h (regs : Blist) (block : Blist) : Blist :=
+    intsToBits (SHA256.hash_block (bitsToInts regs) (bitsToInts block)).
+
+  Definition sha_splitandpad (msg : Blist) : Blist :=
+    bytesToBits (sha_padding_lemmas.pad (bitsToBytes msg)).
+
